Changed input format to remove any quotation marks

examples/mtlr_example/example.py
@@ -9,58 +9,6 @@
 from dafny import *
 import program_loader
 
-seq_2d = Type([], Dafny.SEQ2D)
-seq_simple = Type([], Dafny.SEQ)
-_int_simple = Type([], Dafny.INT)
-
-# seq_2d = Type([seq_2d_simple])  # keep seq_2d simple
-seq = Type([seq_simple])
-_int = Type([_int_simple])
-
-####### recSumS definition #######
-rec_sum_body = """if s == [] then [] else if |s| == 1 then preSum(s[0]) else  
-    vAdd(recSumS(s[..|s|-1]), preSum(s[|s|-1]))"""
-rec_sum_join = """vAdd(a, b)"""
-
-rec_sum = Function("recSumS", ["s"], [seq_2d], seq, [], [],
-                   ["|recSumS(s)| == width(s)"], [], rec_sum_body, rec_sum_join)
-
-####### Mrr definition #######
-mrr_body = """(if s == [] then 0 else if |s| == 1 then vMax(zeroSeq(|s[|s|-1]|), 
-    preSum(s[|s|-1])) else vMax(recSumS(s[..|s|-1]), preSum(s[|s|-1])))"""
-mrr_join = """vMax(a.1, b.1)"""
-
-mrr = Function("Mrr", ["s"], [seq_2d], _int, [], [], [], [rec_sum],
-               mrr_body, mrr_join)
-
-####### Mcr definition #######
-mcr_body = """(if s == [] then []  else if |s| == 1 then preSum(s[0]) else 
-    pMax(recSumS(s), Mcr(s[..|s|-1]).0))"""
-mcr_join = """pMax(vAdd(a.1, b.0), a.0)"""
-
-mcr = Function("Mcr", ["s"], [seq_2d], seq, [], [],
-               ["|Mcr(s).0| == width(s)"], [rec_sum], mcr_body, mcr_join)
-
-####### Mtlr definition #######
-mtlr_body = """(if s == [] then 0 else Max(Mtlr(s[..|s|-1]).0, Mrr(s).0))"""
-mtlr_join = """Max(a.0, vMax(a.1.1, b.1.0))"""
-
-mtlr = Function("Mtlr", ["s"], [seq_2d], _int, [], [], [], [mcr], mtlr_body,
-                mtlr_join)
-
-####### Mblr definition #######
-# Note: this Mblr computes the best bottom-left rectangle of each width
-mblr_body = """(if s == [] then zeroSeq(width(s))
-                else if |s| == 1 then pMax(zeroSeq(|s[|s|-1]|), preSum(s[|s|-1]))
-                else pMax(vAdd(Mblr(s[..|s|-1]).0, preSum(s[|s|-1])),
-                     Mblr([s[|s|-1]]).0 ))"""
-mblr_join = """pMax(vAdd(a.0, b.1), b.0)"""
-
-mblr = Function("Mblr", ["s"], [seq_2d], seq, ["|s|"], [], [], [rec_sum],
-                mblr_body, mblr_join)
-
-all_funcs = [rec_sum, mrr, mcr, mtlr, mblr]
-
 
 def test_printing() -> None:
     program_loader.generate_proof("example_input.txt",
