examples/mtlr_example/output.dfy
@@ -7,7 +7,7 @@ function recSumS(s: seq2D): (seq<int>)
 
 function Mrr(s: seq2D): ((int), (seq<int>))
 {
-    var MrrRes := ((if s == [] then 0 else if |s| == 1 then vMax(zeroSeq(|s[|s|-1]|), preSum(s[|s|-1])) else vMax(recSumS(s[..|s|-1]), preSum(s[|s|-1]))));
+    var MrrRes := (if s == [] then 0 else if |s| == 1 then vMax(zeroSeq(|s[|s|-1]|), preSum(s[|s|-1])) else vMax(recSumS(s[..|s|-1]), preSum(s[|s|-1])));
     var recSumSRes := recSumS(s);
     (MrrRes, recSumSRes)
 }
@@ -15,7 +15,7 @@ function Mrr(s: seq2D): ((int), (seq<int>))
 function Mcr(s: seq2D): ((seq<int>), (seq<int>))
     ensures |Mcr(s).0| == width(s)
 {
-    var McrRes := ((if s == [] then []  else if |s| == 1 then preSum(s[0]) else pMax(recSumS(s), Mcr(s[..|s|-1]).0)));
+    var McrRes := (if s == [] then []  else if |s| == 1 then preSum(s[0]) else pMax(recSumS(s), Mcr(s[..|s|-1]).0));
     var recSumSRes := recSumS(s);
     (McrRes, recSumSRes)
 }
@@ -30,10 +30,10 @@ function Mtlr(s: seq2D): ((int), ((seq<int>), (seq<int>)))
 function Mblr(s: seq2D): ((seq<int>), (seq<int>))
     decreases |s|
 {
-    var MblrRes := ((if s == [] then zeroSeq(width(s))
+    var MblrRes := (if s == [] then zeroSeq(width(s))
                     else if |s| == 1 then pMax(zeroSeq(|s[|s|-1]|), preSum(s[|s|-1]))
                     else pMax(vAdd(Mblr(s[..|s|-1]).0, preSum(s[|s|-1])),
-                         Mblr([s[|s|-1]]).0 )));
+                         Mblr([s[|s|-1]]).0));
     var recSumSRes := recSumS(s);
     (MblrRes, recSumSRes)
 }
